checker/theories/Substitution.v
@@ -1882,8 +1882,7 @@ Proof.
     * eapply All_map.
       eapply (All_impl X0); simpl.
       intros x [u [Hs Hs']]; exists u.
-      specialize (Hs' _ _ _ _ sub eq_refl).
-      now rewrite -map_dtype.
+      now specialize (Hs' _ _ _ _ sub eq_refl).
     * eapply All_map.
       eapply (All_impl X1); simpl.
       intros x [[Hb Hlam] IH].
@@ -1904,8 +1903,7 @@ Proof.
     * eapply All_map.
       eapply (All_impl X0); simpl.
       intros x [u [Hs Hs']]; exists u.
-      specialize (Hs' _ _ _ _ sub eq_refl).
-      now rewrite -map_dtype.
+      now specialize (Hs' _ _ _ _ sub eq_refl).
     * eapply All_map.
       eapply (All_impl X1); simpl.
       intros x [Hb IH].
