pcuic/theories/PCUICInversion.v
@@ -1,15 +1,12 @@
 (* Distributed under the terms of the MIT license.   *)
 From Coq Require Import Bool List.
 From MetaCoq.Template Require Import config utils.
-From MetaCoq.PCUIC Require Import PCUICAst
-     PCUICLiftSubst PCUICUnivSubst PCUICTyping
-     PCUICCumulativity PCUICConversion.
-Local Open Scope string_scope.
+From MetaCoq.PCUIC Require Import PCUICAst PCUICLiftSubst PCUICUnivSubst
+     PCUICTyping PCUICCumulativity PCUICConversion.
 Set Asymmetric Patterns.
-Require Import Equations.Prop.DepElim.
 Import ListNotations.
 
-Set Equations With UIP.
+Require Import Equations.Prop.DepElim.
 
 Section Inversion.
 
