pcuic/theories/PCUICPretty.v
@@ -1,6 +1,6 @@
 (* Distributed under the terms of the MIT license.   *)
 
-From Coq Require Import List Program String.
+From Coq Require Import List String.
 From MetaCoq.Template Require Import utils.
 From MetaCoq.PCUIC Require Import PCUICAst PCUICAstUtils PCUICChecker
      PCUICLiftSubst.
