pcuic/theories/PCUICPrincipality.v
@@ -1,7 +1,7 @@
 (* Distributed under the terms of the MIT license.   *)
 Set Warnings "-notation-overridden".
 
-From Coq Require Import String Bool List Program.
+From Coq Require Import String Bool List.
 From MetaCoq.Template Require Import config utils.
 From MetaCoq.PCUIC Require Import PCUICAst PCUICAstUtils PCUICInduction
      PCUICLiftSubst PCUICTyping PCUICSubstitution PCUICEquality
