template-coq/theories/WfInv.v
@@ -1,7 +1,6 @@
 (* Distributed under the terms of the MIT license.   *)
 
-From Coq Require Import Bool List Program Arith Lia
-     ssreflect ssrbool.
+From Coq Require Import Bool List Arith Lia ssreflect ssrbool.
 From MetaCoq.Template Require Import config utils Ast AstUtils.
 
 
@@ -17,7 +16,7 @@ Fixpoint wf_Inv (t : term) :=
   | tLetIn na t b b' => wf t /\ wf b /\ wf b'
   | tApp t u => isApp t = false /\ u <> nil /\ wf t /\ Forall wf u
   | tConst _ _ | tInd _ _ | tConstruct _ _ _ => True
-  | tCase ci p c brs => wf p /\ wf c /\ Forall (Program.Basics.compose wf snd) brs
+  | tCase ci p c brs => wf p /\ wf c /\ Forall (wf ∘ snd) brs
   | tProj p t => wf t
   | tFix mfix k => Forall (fun def => wf def.(dtype) /\ wf def.(dbody) /\ isLambda def.(dbody) = true) mfix
   | tCoFix mfix k => Forall (fun def => wf def.(dtype) /\ wf def.(dbody)) mfix
@@ -79,7 +78,7 @@ Fixpoint wf_term (t : term) : bool :=
   | tLetIn na t b b' => wf_term t && wf_term b && wf_term b'
   | tApp t u => ~~ isApp t && ~~ is_empty u && wf_term t && forallb wf_term u
   | tConst _ _ | tInd _ _ | tConstruct _ _ _ => true
-  | tCase ci p c brs => wf_term p && wf_term c && forallb (Program.Basics.compose wf_term snd) brs
+  | tCase ci p c brs => wf_term p && wf_term c && forallb (wf_term ∘ snd) brs
   | tProj p t => wf_term t
   | tFix mfix k =>
     forallb (fun def => wf_term def.(dtype) && wf_term def.(dbody) && isLambda def.(dbody)) mfix
